CoC.sml
@@ -1,17 +1,935 @@
 
+
 val _ = new_sort "cat" [];
 
-val _ = new_sort "func" [("A",mk_sort "cat" []),("B",mk_sort "cat" [])]
+val _ = new_sort "fun" [("A",mk_sort "cat" []),("B",mk_sort "cat" [])]
 
-val _ = new_sort_infix "func" "=>"
+val _ = new_sort_infix "fun" "->"
 
 val cat_sort = mk_sort "cat" []
-fun func_sort A B = mk_sort "func" [A,B]
+fun fun_sort A B = mk_sort "fun" [A,B]
 fun mk_cat A = mk_var(A,cat_sort)
-fun mk_func F A B = mk_var(F,func_sort A B)
+fun mk_fun F A B = mk_var(F,fun_sort A B)
 
-val _ = EqSorts := "func" :: (!EqSorts)
+val _ = EqSorts := "fun" :: (!EqSorts)
 
-val _ = new_pred "Holds" [("R",rel_sort (mk_set "A") (mk_set "B")),
-                         ("a",mem_sort (mk_set "A")),
-                         ("b",mem_sort (mk_set "B"))]
+ 
+
+val _ = new_sort "nt" [("f",fun_sort (mk_cat "A") (mk_cat "B")),
+                       ("g",fun_sort (mk_cat "A") (mk_cat "B"))]
+
+
+val _ = new_fun "o" (mk_sort "fun" [mk_var("A",mk_sort "cat" []),mk_var("C",mk_sort "cat" [])],[("f",mk_sort "fun" [mk_var("B",mk_sort "cat" []),mk_var("C",mk_sort "cat" [])]),("g",mk_sort "fun" [mk_var("A",mk_sort "cat" []),mk_var("B",mk_sort "cat" [])])])
+
+
+fun ex2fsym0 name args th = th |> eqT_intro |> iffRL |> ex2fsym name args
+                               |> C mp (trueI []) 
+
+fun uex_expand th = rewr_rule [uex_def $ concl th] th
+
+val isPr_def = define_pred
+“!A B AB p1:AB->A p2:AB->B. isPr(p1,p2) <=>
+   !X f:X->A g:X->B.?!fg:X->AB. p1 o fg = f & p2 o fg = g”
+
+val isPr_ex = store_ax("isPr_ex",“!A B.?AB p1:AB->A p2:AB->B.isPr(p1,p2)”);
+
+val Po_def = isPr_ex |> spec_all |> ex2fsym0 "*" ["A","B"] |> gen_all |> store_as "Po_def"
+
+val p1_def = Po_def |> spec_all |> ex2fsym0 "p1" ["A","B"] |> gen_all |> store_as "p1_def"
+
+val p2_def = p1_def |> spec_all |> ex2fsym0 "p2" ["A","B"] |> gen_all |> store_as "p2_def"
+
+
+val Pa_def = p2_def |> rewr_rule[isPr_def] |> spec_all
+                    |> uex_expand 
+                    |> ex2fsym0 "Pa" ["f","g"] |> gen_all
+                    |> store_as "Pa_def"
+
+val _ = add_parse 0x1D7D8
+
+val _ = add_parse 120793
+
+
+val isEq_def = define_pred
+“!A B f:A->B g E e:E->A. 
+      isEq(f,g,e) <=> 
+      f o e = g o e & 
+      !X a:X->A. f o a = g o a ==>
+      ?!a0:X->E. a = e o a0”
+
+val isEq_ex = store_ax("isEq_ex",“!A B f:A->B g:A->B.?E e:E->A.isEq(f,g,e)”)
+
+val Eqa_def = 
+    isEq_def |> iffLR 
+             |> spec_all |> undisch |> conjE2 
+             |> spec_all |> undisch |> uex_expand
+             |> conj_all_assum |> disch_all
+             |> ex2fsym "Eqa" ["f","g","e","a"]
+             |> gen_all
+             |> store_as "Eqa_def"
+ 
+
+val is0_def = 
+define_pred “!ZERO.is0(ZERO) <=> !X.?!f:ZERO ->X. T”
+
+
+val ZERO_ex = store_ax("ZERO_ex",“?ZERO.is0(ZERO)”)
+
+val ZERO_def = ex2fsym0 "0" [] ZERO_ex |> store_as "ZERO_def"
+
+val ZERO_prop = ZERO_def |> conv_rule (once_depth_fconv no_conv (rewr_fconv (spec_all is0_def))) |> store_as "ZERO_prop"
+
+val From0_def = ZERO_prop |> spec_all |> uex_expand |> ex2fsym0 "From0" ["X"] |> gen_all |> store_as "From0_def"
+
+
+
+val is1_def = define_pred
+“!ONE. is1(ONE) <=> !X.?!f:X->ONE.T”
+
+
+
+val ONE_ex = store_ax("ONE_ex",“?ONE.is1(ONE)”)
+                    
+val ONE_def = ex2fsym0 "1" [] ONE_ex |> store_as "ONE_def"
+
+val ONE_prop = ONE_def |> rewr_rule [is1_def]
+                       |> store_as "ONE_prop"
+
+val To1_def = ONE_prop |> spec_all |> uex_expand |> ex2fsym0 "To1" ["X"] |> gen_all |> store_as "To1_def"
+
+
+
+val _ = new_fun "id" 
+       (mk_sort "fun" [mk_var("A",mk_sort "cat" []),mk_var("A",mk_sort "cat" [])],
+        [("A",mk_sort "cat" [])])
+
+
+val idL = store_ax("idL", “!B A f:B->A. id(A) o f = f”);
+
+val idR = store_ax("idR",“!A B f:A->B. f o id(A) = f”);
+
+val o_assoc = store_ax("o_assoc",“!A.!B.!f: A -> B.!C.!g:B -> C.!D.!h: C -> D.(h o g) o f = h o g o f”);
+
+
+val _ = new_pred "Iso" [("f",fun_sort (mk_cat "A") (mk_cat "B"))]
+
+val Iso_def = store_ax("Iso_def",
+“!A B f:A->B. Iso(f) <=> ?f':B->A. f' o f = id(A) & f o f' = id(B)”);
+
+
+val areIso_def = store_ax("areIso_def",
+“!A B. areIso(A,B) <=> ?f:A->B g:B->A. f o g = id(B) & g o f = id(A)”)
+
+val ZERO_not_ONE = store_ax("ZERO_not_ONE",
+“~(?f:0->1. Iso(f))”)
+
+
+val _ = new_fun "2" (cat_sort,[])
+
+val _ = new_fun "0f" (fun_sort (rastt "1") (rastt "2"),[])
+
+val _ = new_fun "1f" (fun_sort (rastt "1") (rastt "2"),[])
+
+
+val isExp_def = define_pred
+“!A B A2B ev:A * A2B -> B.
+         isExp(ev) <=> !X f:A * X->B. ?!h:X->A2B. ev o Pa(p1(A,X), h o p2(A,X)) = f”
+
+
+
+
+val isExp_ex = store_ax("isExp_ex",“!A B. ?A2B ev:A * A2B->B. isExp(ev)”);
+
+val Exp_def = isExp_ex |> spec_all 
+                       |> ex2fsym0 "Exp" ["A","B"] |> gen_all
+                       |> store_as "Exp_def"
+
+val Ev_def = Exp_def |> spec_all |> rewr_rule[isExp_def]
+                     |> ex2fsym0 "Ev" ["A","B"]
+                     |> gen_all
+                     |> store_as "Ev_def"
+
+val Tp_def = Ev_def |> spec_all |> uex_expand 
+                    |> ex2fsym0 "Tp" ["f"] |> gen_all
+                    |> store_as "Tp_def"
+
+
+val _ = new_pred "isPb"
+  [("f",fun_sort (mk_cat "X") (mk_cat "Z")),
+   ("g",fun_sort (mk_cat "Y") (mk_cat "Z")),
+   ("p",fun_sort (mk_cat "P") (mk_cat "X")),
+   ("q",fun_sort (mk_cat "P") (mk_cat "Y"))];
+
+
+val isPb_def = store_ax("isPb_def",
+“!X H f:X -> H Y g : Y -> H P p : P -> X q : P -> Y.
+ isPb(f, g, p, q) <=> f o p = g o q &
+ !A u : A -> X v : A -> Y. 
+    f o u = g o v ==> 
+    ?!a : A -> P. p o a = u & q o a = v”);
+
+val isPb_expand = isPb_def
+                      |> conv_rule $ once_depth_fconv no_conv (rewr_fconv $ uex_def “?!a : A -> P. p:P->X o a = u & q:P->Y o a = v”) |> store_as "isPb_expand";
+
+val isPb_ex = store_ax("isPb_ex",“!X H f:X->H Y g:Y->H. ?P p:P->X q. isPb(f,g,p,q)”);
+
+val PCC1 = store_ax("PCC1",
+“?p:0->1 q:0->1. isPb(0f,1f,p,q)”);
+
+val CC2_2 = store_ax("CC2_2",
+“!A B f:A->B g:A->B. ~(f = g) ==> ?a:2->A. ~(f o a = g o a)”);
+
+
+val imp_lemma = proved_th $
+e0
+(dimp_tac >> strip_tac (* 3 *)
+ >-- (cases_on “A” >-- arw[] >> first_x_assum drule >>
+      arw[]) >>
+ arw[])
+(form_goal
+ “~ A ==> B <=> B | A”)
+
+val uex_tac:tactic = fn (ct,asl,w) =>
+    let val th = uex_def w
+        val w' = snd $ dest_dimp $ concl th
+    in ([(ct,asl,w')],(sing (dimp_mp_r2l th)))
+    end
+ 
+val Thm1 = prove_store("Thm1",
+e0
+(strip_tac >> cases_on “0f o To1(C) = 1f o To1(C)” 
+ >-- (strip_assume_tac PCC1 >> fs[isPb_def] >>
+      first_x_assum rev_drule >>
+      pop_assum (strip_assume_tac o uex_expand) >>
+      qsuff_tac ‘~(?a1 : 2->C. T) ==> is0(C)’
+      >-- rw[imp_lemma] >>
+      strip_tac >> rw[is0_def] >> strip_tac >> uex_tac >>
+      qexists_tac ‘From0(X) o a’ >> rw[] >> rpt strip_tac >>
+      ccontra_tac >> drule CC2_2 >> fs[] >>
+      qsuff_tac ‘?a1:2->C.T’ >-- (rw[] >>
+      first_x_assum accept_tac) >>
+      qexists_tac ‘a'’ >> rw[]) >>
+ disj2_tac >> drule CC2_2 >> 
+ pop_assum strip_assume_tac >> qexists_tac ‘a’ >> rw[])
+(form_goal
+ “!C. is0(C) | (?a:2->C.T)”) );
+
+val iscoPr_def = define_pred
+“!A B AB i1:A->AB i2:B->AB. iscoPr(i1,i2) <=>
+   !X f:A->X g:B->X.?!fg:AB->X.fg o i1 = f & fg o i2 = g”
+
+
+
+
+val iscoPr_ex = store_ax("iscoPr_ex",“!A B.?AB i1:A->AB i2:B->AB.iscoPr(i1,i2)”);
+
+val coPo_def = iscoPr_ex |> spec_all |> ex2fsym0 "+" ["A","B"] |> gen_all |> store_as "coPo_def";
+
+val i1_def = coPo_def |> spec_all |> ex2fsym0 "i1" ["A","B"] |> gen_all |> store_as "i1_def";
+
+val i2_def = i1_def |> spec_all |> ex2fsym0 "i2" ["A","B"] |> gen_all |> store_as "i2_def";
+
+val coPa_def = i2_def |> rewr_rule[iscoPr_def] |> spec_all
+                      |> uex_expand 
+                      |> ex2fsym0 "coPa" ["f","g"]
+                      |> gen_all
+                      |> store_as "coPa_def";
+
+
+val _ = new_pred "Mono" [("f",fun_sort (mk_cat "A") (mk_cat "B"))]
+
+val Mono_def = store_ax("Mono_def",“!A B f:A->B. Mono(f) <=> !X g:X->A h. f o g = f o h ==> g = h”);
+
+val rfs = rev_full_simp_tac
+
+val post_inv_Mono = prove_store("post_inv_Mono",
+e0
+(rpt strip_tac >> rw[Mono_def] >> rpt strip_tac >>
+ qby_tac
+ ‘i o m o g = i o m o h’ >-- arw[] >>
+ rfs[GSYM o_assoc] >> fs[idL])
+(form_goal
+ “!A B m:A->B i:B->A. i o m = id(A) ==> Mono(m)”));
+
+
+
+val i12_of_coPa = coPa_def |> spec_all |> conjE1
+                           |> gen_all 
+                           |> store_as "i12_of_coPa";
+
+val i1_of_coPa = i12_of_coPa |> spec_all |> conjE1
+                             |> gen_all 
+                             |> store_as "i1_of_coPa";
+
+
+val i2_of_coPa = i12_of_coPa |> spec_all |> conjE2
+                             |> gen_all 
+                             |> store_as "i2_of_coPa";
+ 
+val Thm2_1_i1 = prove_store("Thm2_1_i1",
+e0
+(rpt strip_tac >> rw[Mono_def] >> rpt strip_tac >>
+ cases_on “g:X->A = h” >-- arw[] >>
+ qsuff_tac ‘?f:B->A.T’
+ >-- (strip_tac >> 
+      qby_tac ‘coPa(id(A),f) o i1(A,B) = id(A)’
+      >-- rw[i1_of_coPa] >>
+      qby_tac ‘coPa(id(A),f) o i1(A, B) o g = coPa(id(A),f) o i1(A, B) o h’
+      >-- arw[] >>
+      rfs[GSYM o_assoc,idL]) >>
+ drule CC2_2 >> pop_assum strip_assume_tac >>
+ qexists_tac ‘g o a o 1f o To1(B)’ >> rw[])
+(form_goal
+ “!A B. Mono(i1(A,B))”));
+
+
+val to1_unique = prove_store("to1_unique",
+e0
+(rpt strip_tac >>
+ qspecl_then [‘X’,‘f’] assume_tac To1_def >>
+ qspecl_then [‘X’,‘g’] assume_tac To1_def >> 
+ arw[])
+(form_goal
+ “!X f:X->1 g:X->1. f = g”));
+
+val one_to_one_id = prove_store("one_to_one_id",
+e0
+(strip_tac >>
+ qspecl_then [‘1’,‘f’,‘id(1)’] assume_tac to1_unique >>
+ first_x_assum accept_tac)
+(form_goal
+ “!f:1->1. f = id(1)”))
+
+val from0_unique = prove_store("form0_unique",
+e0
+(rpt strip_tac >>
+ qspecl_then [‘X’,‘f’] assume_tac From0_def >>
+ qspecl_then [‘X’,‘g’] assume_tac From0_def >> 
+ arw[])
+(form_goal
+ “!X f:0->X g:0->X. f = g”));
+
+val zero_to_zero_id = prove_store("zero_to_zero_id",
+e0
+(strip_tac >>
+ qspecl_then [‘0’,‘f’,‘id(0)’] assume_tac from0_unique >>
+ first_x_assum accept_tac)
+(form_goal
+ “!f:0->0. f = id(0)”))
+
+
+val one_not_to_zero = prove_store("one_not_to_zero",
+e0
+(strip_tac >> assume_tac ZERO_not_ONE >>
+ qsuff_tac ‘?g:0->1. Iso(g)’ >-- arw[] >>
+ pop_assum (K all_tac) >>
+ rw[Iso_def] >> qexistsl_tac [‘From0(1)’,‘f’] >>
+ rw[zero_to_zero_id,one_to_one_id])
+(form_goal “!f:1->0.F”));
+
+
+val to0_is0 = prove_store("to0_is0",
+e0
+(rw[is0_def] >> rpt strip_tac >> uex_tac >>
+ qexists_tac ‘From0(X) o f0’ >> rw[] >> rpt strip_tac >>
+ ccontra_tac >> drule CC2_2 >> pop_assum strip_assume_tac >>
+ qsspecl_then [‘f0 o a o 1f’] assume_tac one_not_to_zero >> 
+ first_x_assum accept_tac)
+(form_goal
+ “!A f0:A->0. is0(A)”));
+
+val Thm2_2 = prove_store("Thm2_2",
+e0
+(rw[isPb_def] >> rpt strip_tac >> strip_assume_tac PCC1 >>
+ fs[isPb_def] >> 
+ qsuff_tac ‘?u:P->1 v. 0f o u = 1f o v’
+ >-- (strip_tac >> first_x_assum drule >> 
+      pop_assum (strip_assume_tac o uex_expand) >>
+      qsspecl_then [‘a’] accept_tac to0_is0) >> 
+ qexistsl_tac [‘To1(A) o p’,‘To1(B) o q’] >>
+ qby_tac 
+  ‘coPa(0f o To1(A), 1f o To1(B)) o i1(A, B) o p = 
+   coPa(0f o To1(A), 1f o To1(B)) o i2(A, B) o q’ 
+ >-- arw[] >>
+ fs[GSYM o_assoc,i12_of_coPa])
+(form_goal
+ “!A B P p:P->A q.isPb(i1(A,B),i2(A,B),p,q) ==> is0(P)”));
+
+val Epi_def = store_ax("Epi_def",“!A B f:A->B. Epi(f) <=> !X g:B->X h. g o f = h o f ==> g = h”);
+
+val CC3 = store_ax("CC3", “~Epi(coPa(0f,1f))”);
+
+val isgen_def = define_pred
+“!G. isgen(G) <=> !A B f1:A->B f2. ~(f1 = f2) ==> ?g: G -> A. ~(f1 o g = f2 o g)”
+
+
+val isPb_def = store_ax("isPb_def",
+“!X Z f:X -> Z Y g : Y -> Z  P p : P -> X q : P -> Y.
+ isPb(f, g, p, q) <=> f o p = g o q &
+ !A u : A -> X v : A -> Y. 
+    f o u = g o v ==> 
+    ?!a : A -> P. p o a = u & q o a = v”);
+
+
+
+val Thm3_1 = prove_store("Thm3_1",
+e0
+(rpt strip_tac >> fs[isgen_def] >>
+ cheat
+ )
+(form_goal
+ “!G. isgen(G) ==> ?s:2->G r:G->2. r o s = id(2)”));
+
+(*all distinct*)
+
+val Thm3_2 = prove_store("Thm3_2",
+e0
+(cheat)
+(form_goal
+ “!G. isGen(G) & 
+  ?g1 g2 g3:G->G. ~(g1 = g2) & 
+                  ~(g1 = g3) &
+                  ~(g2 = g3) & 
+  !g:G->G. g = g1 | g = g2 | g = g3”));
+
+
+val _ = new_pred "isPo"
+  [("f",fun_sort (mk_cat "Z") (mk_cat "X")),
+   ("g",fun_sort (mk_cat "Z") (mk_cat "Y")),
+   ("p",fun_sort (mk_cat "X") (mk_cat "P")),
+   ("q",fun_sort (mk_cat "Y") (mk_cat "P"))];
+
+
+val isPo_def = store_ax("isPo_def",
+“!H X f:H -> X Y g : H -> Y P p : X -> P q : Y -> P.
+ isPo(f, g, p, q) <=> p o f = q o g &
+ !A u : X -> A v : Y -> A. 
+    u o f = v o g ==> 
+    ?!a : P -> A. a o p = u & a o q = v”);
+
+val isPo_expand = isPo_def
+                      |> conv_rule $ once_depth_fconv no_conv (rewr_fconv $ uex_def “?!a : P -> A. a o p:X->P = u & a o q:Y->P = v”) |> store_as "isPo_expand";
+
+val isPo_ex = store_ax("isPo_ex",“!H X f:H->X Y g:H->Y. ?P p:X->P q:Y->P. isPo(f,g,p,q)”);
+
+
+val _ = new_fun "3" (cat_sort,[])
+
+val _ = new_fun "α" (fun_sort (rastt "2") (rastt "3"),[])
+
+val _ = new_fun "β" (fun_sort (rastt "2") (rastt "3"),[])
+
+
+val _ = new_fun "γ" (fun_sort (rastt "2") (rastt "3"),[])
+
+(*
+And y: 2 -*3 with y 0 0 = a 0 O and y a 1 = ,B a 1. This completes the axiom.
+ The functor F: 3 2 with F a = 0 and F o /3 = 2 proves L i /3. The domain and
+ codomain relations show neither a nor ,B equals y.
+*)
+
+val CC4_1 = store_ax("CC4_1",
+“γ o 0f = α o 0f & γ o 1f = β o 1f”)
+
+val CC4_2 = store_ax("CC4_2",“isPo(1f,0f,α,β)”)
+
+val Poa_def = 
+    isPo_expand |> iffLR 
+                |> strip_all_and_imp
+                |> conjE2
+                |> strip_all_and_imp
+                |> ex2fsym0 
+                "Poa" ["f","g","p","q","u","v"]
+                |> disch 
+                “u:X->A o f:H->X = v:Y->A o g”
+                |> qgenl [‘A’,‘u’,‘v’]
+                |> disch_all
+                |> qgenl
+                [‘H’,‘X’,‘f’,‘Y’,‘g’,‘P’,‘p’,‘q’]
+
+val oa_ex = prove_store("oa_ex",
+e0
+(rpt strip_tac >> 
+ qexists_tac ‘Poa(1f,0f,α,β,f,g) o γ’ >>
+ rw[])
+(form_goal
+ “!A f:2->A g. f o 1f = g o 0f ==> 
+  ?gf:2->A. gf = Poa(1f,0f,α,β,f,g) o γ”));
+  
+ 
+val oa_def = oa_ex |> spec_all |> undisch 
+                   |> ex2fsym0 "@" ["g","f"]
+
+
+(* THEOREM 4. The composite in 2 of the nonidentity arrow 12 with either of the
+ identity arrows 0 ? !2 and 0 a !2 is 1*)
+
+
+val zero_ex = prove_store("zero_ex",
+e0
+cheat
+(form_goal
+ “∃z:2->2. z = 0f o To1(2)”));  
+
+val zero_def = zero_ex |> ex2fsym0 "𝟘" [] 
+
+
+val one_ex = prove_store("one_ex",
+e0
+cheat
+(form_goal
+ “∃l:2->2. l = 1f o To1(2)”));  
+
+val one_def = one_ex |> ex2fsym0 "𝟙" [] 
+
+val Thm4 = prove_store("Thm4",
+e0
+cheat
+(form_goal “𝟙 @ id(2) = id(2) & 
+            id(2) o 𝟘 = id(2)”)
+)
+
+
+val dom_ex = prove_store("dom_ex",
+e0
+(cheat)
+(form_goal
+“!A f:2->A. ?df. df = f o 0f”));
+
+val dom_def = dom_ex |> spec_all |> ex2fsym0 "dom" ["f"]
+                     |> gen_all
+
+val cod_ex = prove_store("cod_ex",
+e0
+(cheat)
+(form_goal
+“!A f:2->A. ?df. df = f o 1f”));
+
+val cod_def = cod_ex |> spec_all |> ex2fsym0 "cod" ["f"]
+                     |> gen_all
+
+
+(*composable*)
+val cpsb_def = define_pred “!A f:2->A g:2->A. cpsb(g,f) <=> dom(g) = cod(f)”;
+
+val isid_def = define_pred “!A f:2->A. isid(f) <=> ?f0:1->A. f = f0 o To1(2)”
+
+val Thm5 = prove_store("Thm5",
+e0
+(cheat)
+(form_goal
+ “!A f:2->A. isid(f) ==> 
+  (!g. cpsb(g,f) ==> g @ f = g) & 
+  (!g. cpsb(f,g) ==> f @ g = g)”));
+
+
+
+val Tp0_ex = prove_store("Tp0_ex",
+e0
+(rpt strip_tac >> qexists_tac ‘Ev(X,Y) o Pa(id(X),f o To1(X))’ >>
+ rw[])
+(form_goal
+ “!X Y f:1->Exp(X,Y).?tp0:X->Y. Ev(X,Y) o Pa(id(X),f o To1(X)) = tp0”));
+
+val Tp0_def = 
+    Tp0_ex |> spec_all |> ex2fsym0 "Tp0" ["f"] |> gen_all
+           |> store_as "Tp0_def"
+
+
+
+val Swap_ex = proved_th $
+e0
+(rpt strip_tac >> qexists_tac ‘Pa(p2(A,B),p1(A,B))’ >> rw[])
+(form_goal
+ “!A B. ?swap:A * B ->B * A. Pa(p2(A,B),p1(A,B)) = swap”)
+
+val Swap_def = 
+    Swap_ex |> spec_all |> eqT_intro
+               |> iffRL |> ex2fsym "Swap" ["A","B"] 
+               |> C mp (trueI []) |> gen_all
+               |> store_as "Swap_def";
+
+val p12_of_Pa = Pa_def |> spec_all |> conjE1
+                       |> gen_all
+                       |> store_as "p12_of_Pa";
+
+
+val Swap_property = proved_th $
+e0
+(rw[GSYM Swap_def,p12_of_Pa])
+(form_goal
+ “!A B. p1(B,A) o Swap(A,B) = p2(A,B) & p2(B,A) o Swap(A,B) = p1(A,B)”)
+
+
+val is_Pa = Pa_def |> spec_all |> conjE2 |> gen_all
+                   |> store_as "is_Pa";
+
+val to_P_component = prove_store("to_Pr_component",
+e0
+(rpt strip_tac >> irule is_Pa >> rw[])
+(form_goal
+ “!A B X f:X->A * B.  f = Pa(p1(A,B) o f,p2(A,B) o f)”));
+
+val to_P_eq = prove_store("to_P_eq",
+e0
+(rpt strip_tac >>
+ qsuff_tac ‘f = Pa(p1(A,B) o g,p2(A,B) o g) &
+            g = Pa(p1(A,B) o g,p2(A,B) o g)’ >--
+ (strip_tac >> once_arw[] >> rw[]) >>
+ strip_tac (* 2 *) >--
+ (irule is_Pa >> arw[]) >> once_rw[to_P_component])
+(form_goal
+ “!A B X f:X->A * B g:X->A * B. p1(A,B) o f = p1(A,B) o g &
+ p2(A,B) o f = p2(A,B) o g ==> f = g”));
+
+
+val Pa_distr = proved_th $
+e0
+(rpt strip_tac >> irule is_Pa >>
+ rw[GSYM o_assoc,p12_of_Pa])
+(form_goal
+“!A B X a1:X ->A a2:X->B X0 x:X0->X. Pa(a1,a2) o x = 
+Pa(a1 o x,a2 o x) ”)
+
+val Swap_Swap_id = prove_store("Swap_Swap_id",
+e0
+(rpt strip_tac >> irule to_P_eq >> rw[GSYM Swap_def,idR] >>
+ rw[Pa_distr,p12_of_Pa])
+(form_goal
+ “!A B. Swap(B,A) o Swap(A,B) = id(A * B)”));
+
+(*
+
+val Thm6_square= prove_store("Thm6_sqaure",
+e0
+()
+(form_goal
+ “!fgij:2 * 2 -> A ghkl:2 * 2 -> A f g i j h k l.
+   fgij o Pa(0f o To1(2),id(2)) = f &
+   fgij o Pa(1f o To1(2),id(2)) = g &
+   fgij o Pa(id(2),0f o To1(2)) = i &
+   fgij o Pa(id(2),1f o To1(2)) = j &
+   ghkl o Pa(0f o To1(2),id(2)) = g &
+   ghkl o Pa(1f o To1(2),id(2)) = h &
+   ghkl o Pa(id(2),0f o To1(2)) = k &
+   ghkl o Pa(id(2),1f o To1(2)) = l ==>
+   
+   
+  fgij o Pa(1f o To1(2),id(2)) = f 
+  ghkl o Pa(0f o To1(2),id(2)) & 
+  !cmp:2 * 2 ->A. 
+  cmp o Pa(0f o To1(2),id(2)) = 
+
+  cpsb(ghkl,fgij) ==> 
+  Tp0(ghkl @ fgij) o Pa(id(2),0f o To1(2)) = 
+  (Tp0(ghkl) o Pa(id(2),0f o To1(2))) @ ”));
+
+
+val Thm6 = prove_store("Thm6",
+e0
+()
+(form_goal
+ “!fgij:2-> Exp(2,A) ghkl:2-> Exp(2,A). 
+  cpsb(ghkl,fgij) ==> 
+  Tp0(ghkl @ fgij) o Pa(id(2),0f o To1(2)) = 
+  (Tp0(ghkl) o Pa(id(2),0f o To1(2))) @ ”));
+
+*)
+
+val two_ex = prove_store("two_ex",
+e0
+cheat
+(form_goal
+ “∃t:2->2. t = id(2)”));
+
+val two_def = two_ex |> ex2fsym0 "𝟚" [];
+
+val _ = add_parse (int_of "𝟚");
+(*commutative square*)
+
+val csL_ex = prove_store("csL_ex",
+e0
+(cheat)
+(form_goal
+ “!A cs:2 * 2 ->A. 
+  ∃l. l = cs o Pa(𝟘,𝟚)”));
+
+val csL_def = csL_ex |> spec_all |> ex2fsym0 "csL" ["cs"]
+                     |> gen_all
+
+val csR_ex = prove_store("csR_ex",
+e0
+(cheat)
+(form_goal
+ “!A cs:2 * 2 ->A. 
+  ∃r. r = cs o Pa(𝟙,𝟚)”));
+
+
+val csR_def = csR_ex |> spec_all |> ex2fsym0 "csR" ["cs"]
+                     |> gen_all
+
+
+val csT_ex = prove_store("csT_ex",
+e0
+(cheat)
+(form_goal
+ “!A cs:2 * 2 ->A. 
+  ∃t.t  = cs o Pa(𝟚,𝟘)”));
+
+val csT_def = csT_ex |> spec_all |> ex2fsym0 "csT" ["cs"]
+                     |> gen_all
+
+val csB_ex = prove_store("csB_ex",
+e0
+(cheat)
+(form_goal
+ “!A cs:2 * 2 ->A. 
+  ∃b. b = cs o Pa(𝟚,𝟙)”));
+
+val csB_def = csB_ex |> spec_all |> ex2fsym0 "csB" ["cs"]
+                     |> gen_all
+
+val Thm7 = prove_store("Thm7",
+e0
+cheat
+(form_goal
+ “!A f:2->A g f' g'. 
+   cpsb(g,f) & cpsb(g',f') & 
+   g @ f = g' @ f' ==>
+   ?q: 2* 2->A.
+   csT(q) = f & 
+   csR(q) = g &
+   csL(q) = f' &
+   csB(q) = g'  
+   ”));
+
+
+val iso_def = define_pred
+“!A f:2->A. iso(f) <=> 
+ ?g:2->A. dom(g) = cod(f) & dom(f) = cod(g) &
+ g @ f = dom(f) o To1(2) & f @ g = cod(f) o To1(2) ”
+
+
+val CC6 = store_ax("CC6",
+“?A f:2->A. iso(f) & ~isid(f)”); 
+
+val Thm14 = prove_store("Thm14",
+e0
+cheat
+(form_goal
+“?A A1:1->A A2. ~(A1 = A2) &
+?f:2->A. dom(f) = A1 & cod(f) = A2 ”));
+
+val Thm15 = prove_store("Thm15",
+e0
+cheat
+(form_goal
+ “!A B f:A->B. Epi(f) ==> !B0:1->B. ?A0:1->A. B0 = f o A0”))
+ 
+val Thm16 = prove_store("Thm16",
+e0
+cheat
+(form_goal
+ “!A B f:2->A + B. (?f0:2->A. f = i1(A,B) o f0) |
+(?f0:2->B. f = i2(A,B) o f0)”));
+
+
+(*
+A full subcategory of A is a monic i: S >-4 A such that if f a 0 and f a I are both
+ in S then so is f. A full subcategory classifier is a category Cl with a selected object
+ t: 1 -+ Cl such that any full subcategory i: S >-4 A is the pullback of t along a unique
+ functor c: A - Cl.
+*)
+
+
+val FSC_def = define_pred
+“!S A i:S->A. FSC(i) <=> Mono(i) & 
+ !f:2->A d:1->S c:1->S. dom(f) = i o d & cod(f) = i o c ==> 
+ ?f0:2->S. f = i o f0”;
+
+val FSCC_def = define_pred
+“!Cl t:1->Cl. FSCC(t) <=> 
+ (!S A i:S->A. FSC(i) ==> ?!c:A->Cl. isPb(c,t,i,To1(S)))”
+
+ 
+val Thm17 = prove_store("Thm17",
+e0
+cheat
+(form_goal “?Cl t:1->Cl. FSCC(t)”));
+
+val DC_def = define_pred “!A. DC(A) <=> !f:2->A. isid(f)”
+
+
+
+val iscoEq_def = define_pred
+“!A B f:A->B g cE ce:B -> cE. 
+      iscoEq(f,g,ce) <=> 
+      ce o f = ce o g & 
+      !X x:B->X. x o f = x o g ==>
+      ?!x0:cE->X. x = x0 o ce”
+
+
+
+val iscoEq_ex = store_ax("iscoEq_ex",“!A B f:A->B g:A->B.?cE ce:B->cE.iscoEq(f,g,ce)”);
+
+val coEqa_def = 
+    iscoEq_def |> iffLR 
+               |> spec_all |> undisch |> conjE2 
+               |> spec_all |> undisch |> uex_expand
+               |> conj_all_assum |> disch_all
+               |> ex2fsym "coEqa" ["f","g","ce","x"]
+               |> store_as "coEqa_def"
+
+ 
+val Thm20 = prove_store("Thm20",
+e0
+cheat
+(form_goal
+ “!D. DC(D) ==> !A f:A->D g Q q:D->Q. iscoEq(f,g,q) ==>
+ DC(Q)”));
+ 
+val Thm21 = prove_store("Thm21",
+e0
+cheat
+(form_goal
+ “!A. DC(A) ==> !S i:S->A. FSC(i) ==>
+  ?!c:A-> 1+1. isPb(c,i2(1,1),i,To1(S))
+  ”));
+
+val SO_def = define_pred
+“!A S s:S->A. SO(s) <=> 
+ (DC(S) & Mono(s) & 
+  !X f:X->A. DC(X) ==> ?f0:X->S. f = s o f0)”
+
+val SA_def = define_pred
+“!A S s:S -> Exp(2,A). SA(s) <=> SO(s)”
+
+(*
+ THEOREM 22. If A has a set of objects, so does the coequalizer of any parallel pair with codomain A.
+
+*)
+
+val Thm22 = prove_store("Thm22",
+e0
+cheat
+(form_goal
+ “!A S s:S->A. SO(s) ==> 
+  !X f:X->A g Q q:A->Q. iscoEq(f,g,q) ==>
+  ?Sq sq:Sq -> Q. SO(q)”));
+
+
+(*
+val Thm23 = prove_store("Thm23",
+e0
+()
+(form_goal
+ “”));
+*)
+
+val ICat_def = define_pred
+“∀C0 C1 s: C1-> C0 t:C1 -> C0 e: C0 -> C1 CC c: CC -> C1. 
+ ICat(s,t,e,c) ⇔ 
+ s o e = id(C0) ∧ t o e = id(C0)”
+
+(*
+THEOREM 24. If G: A2 -+ B2 and F: A -+ B are an internal functor between the
+ internal categories on A and B, then G = F
+*)
+val IFun_def = define_pred
+“∀F0:C0 -> D0 F1:C1->D1. IFun(F0,F1) ⇔
+ ”
+
+!A B. A = B <=> 
+ (!X f:X->A. P(f)) <=> (!X f:X->B. P(f)) & 
+ (!X f:A->X. P(f)) <=> (!X f:B->X. P(f))
+
+
+val _ = 
+“?C. ”
+val Z2_O2_ex
+
+
+
+
+IsTopos(C) ==> hasProd(C)
+
+
+?C.
+(asob(A:Ob(C))):ob 
+
+asOb() 
+
+?ETCS. 
+!A B f:A->B. ?
+
+
+
+!C \equiv to the WS of ETCS
+  P()
+
+
+
+
+IsTopos(ETCS) ==> hasProd(ETCS)
+
+!A:OB(ETCS) B.? AB: OB(ETCS)....
+
+
+
+!A:ob B:ob. 
+
+
+
+
+
+cat sort
+fun sort
+
+C:cat
+
+f: C:cat ->D
+
+1 
+
+2
+
+a --> b
+
+C
+
+
+f(a) --> f(b)
+
+
+!f:2->C g:2->C. f o 1 = g o 0 ==>
+ ?! fog: 2->C. fog o 0 = f o 0 &
+               fog o 1 = g o 1
+
+
+!f:2->C g:2->C h:2->C.
+
+f o 1 = g o 0 & ... ==> 
+(h o_C g) o_C f = h o_C g o_C f =
+
+
+
+Ob(C) Ar: Ob(C) -> Ob(C)
+
+
+perfectoid space
+
+fragile
+
+IsTopos(C) ==> hasProd(C)
+
+
+
+
+
+
+
+
+
+
+
+
